thys/LLL_Basis_Reduction/LLL_Integer_Equations.thy
@@ -1,0 +1,344 @@
+(*
+    Authors:    René Thiemann
+    License:    BSD
+*)
+subsection \<open>LLL Implementation based on Integer Arithmetic\<close>
+
+text \<open>In this part we aim to update the integer values $d\,(j+1) * \mu_{i,j}$ as well as the 
+  Gramian determinants $d\,i$. \<close>
+
+subsubsection \<open>Updates of the integer values for Swap, Add, etc.\<close>
+
+text \<open>We provide equations how to implement the LLL-algorithm by storing the integer values
+  $d\, (j+1) * \mu_{i,j}$ and all $d\ i$ in addition to the vectors in $f$.
+  Moreover, we show how to check condition like the one on norms via the integer values.\<close>
+
+theory LLL_Integer_Equations
+  imports LLL
+   LLL_Number_Bounds
+begin
+
+lemma division_to_div: "rat_of_int x = of_int y / of_int z \<Longrightarrow> x = y div z" 
+  by (metis floor_divide_of_int_eq floor_of_int)
+
+lemma int_via_rat_eqI: "rat_of_int x = rat_of_int y \<Longrightarrow> x = y" by auto
+
+hide_fact (open) Word.inc_i
+
+definition floor_ceil_num_denom :: "int \<Rightarrow> int \<Rightarrow> int" where
+  "floor_ceil_num_denom n d = ((2 * n + d) div (2 * d))" 
+
+lemma floor_ceil_num_denom: "denom > 0 \<Longrightarrow> floor_ceil_num_denom num denom = 
+  floor_ceil (of_int num / rat_of_int denom)" 
+  unfolding floor_ceil_def floor_ceil_num_denom_def
+  unfolding floor_divide_of_int_eq[where ?'a = rat, symmetric]
+  by (rule arg_cong[of _ _ floor], simp add: add_divide_distrib)
+
+context LLL
+begin
+
+definition "d\<mu> fs i j = int_of_rat (of_int (d fs (Suc j)) * \<mu> fs i j)" 
+
+lemma d\<mu>: assumes inv: "LLL_invariant upw i fs" "j < ii" "ii < m" 
+  shows "of_int (d\<mu> fs ii j) = of_int (d fs (Suc j)) * \<mu> fs ii j" 
+  unfolding d\<mu>_def using LLL_mu_d_Z[OF inv] by auto
+
+lemma d_sq_norm_comparison: assumes inv: "LLL_invariant upw k fs" 
+  and quot: "quotient_of \<alpha> = (num,denom)" 
+  and i: "i < m" 
+  and i0: "i \<noteq> 0" 
+  shows "(d fs i * d fs i * denom \<le> num * d fs (i - 1) * d fs (Suc i))
+   = (sq_norm (gso fs (i - 1)) \<le> \<alpha> * sq_norm (gso fs i))" 
+proof -
+  let ?r = "rat_of_int" 
+  let ?x = "sq_norm (gso fs (i - 1))" 
+  let ?y = "\<alpha> * sq_norm (gso fs i)" 
+  from i have le: "i - 1 \<le> m" " i \<le> m" "Suc i \<le> m" by auto
+  note pos = LLL_d_pos[OF inv le(1)] LLL_d_pos[OF inv le(2)] quotient_of_denom_pos[OF quot]
+  have "(d fs i * d fs i * denom \<le> num * d fs (i - 1) * d fs (Suc i))
+    = (?r (d fs i * d fs i * denom) \<le> ?r (num * d fs (i - 1) * d fs (Suc i)))" (is "?cond = _") by presburger
+  also have "\<dots> = (?r (d fs i) * ?r (d fs i) * ?r denom \<le> ?r num * ?r (d fs (i - 1)) * ?r (d fs (Suc i)))" by simp
+  also have "\<dots> = (?r (d fs i) * ?r (d fs i) \<le> \<alpha> * ?r (d fs (i - 1)) * ?r (d fs (Suc i)))" 
+    using pos unfolding quotient_of_div[OF quot] by (auto simp: field_simps)
+  also have "\<dots> = (?r (d fs i) / ?r (d fs (i - 1)) \<le> \<alpha> * (?r (d fs (Suc i)) / ?r (d fs i)))" 
+    using pos by (auto simp: field_simps)
+  also have "?r (d fs i) / ?r (d fs (i - 1)) = ?x" using LLL_d_Suc[OF inv, of "i - 1"] pos i i0
+    by (auto simp: field_simps)
+  also have "\<alpha> * (?r (d fs (Suc i)) / ?r (d fs i)) = ?y" using LLL_d_Suc[OF inv i] pos i i0
+    by (auto simp: field_simps)
+  finally show "?cond = (?x \<le> ?y)" .
+qed
+
+lemma floor_ceil_num_denom_d\<mu>_d: assumes inv: "LLL_invariant upw k fs"
+  and j: "j < i" and i: "i < m"  
+shows "floor_ceil_num_denom (d\<mu> fs i j) (d fs (Suc j)) = floor_ceil (\<mu> fs i j)" 
+proof -
+  from j i have sj: "Suc j \<le> m" by auto
+  note pos = LLL_d_pos[OF inv sj]
+  show ?thesis unfolding floor_ceil_num_denom[OF pos]
+    by (rule arg_cong[of _ _ floor_ceil], subst d\<mu>[OF inv j i], insert pos, auto)
+qed
+
+lemma d_d\<mu>_add_row: assumes Linv: "LLL_invariant True i fs"
+  and i: "i < m"  and j: "j < i" 
+  and c: "c = floor_ceil (\<mu> fs i j)" 
+  and fs': "fs' = fs[ i := fs ! i - c \<cdot>\<^sub>v fs ! j]" 
+  and mu_small: "\<mu>_small_row i fs (Suc j)" 
+shows  
+  (* d-updates: none *)
+  "\<And> ii. ii \<le> m \<Longrightarrow> d fs' ii = d fs ii" 
+  (* d\<mu>-updates: *)
+  "\<And> i' j'. i' < m \<Longrightarrow> j' < i' \<Longrightarrow>       
+     d\<mu> fs' i' j' = (
+       if i' = i \<and> j' < j 
+         then d\<mu> fs i' j' - c * d\<mu> fs j j' 
+       else if i' = i \<and> j' = j 
+         then d\<mu> fs i' j' - c * d fs (Suc j) 
+       else d\<mu> fs i' j')"
+    (is "\<And> i' j'. _ \<Longrightarrow> _ \<Longrightarrow> _ = ?new_mu i' j'")
+proof -
+  note add = basis_reduction_add_row_main[OF Linv i j c fs' mu_small]
+  show d: "\<And> ii. ii \<le> m \<Longrightarrow> d fs' ii = d fs ii" by fact
+  fix i' j'
+  assume i': "i' < m" and j': "j' < i'"   
+  hence j'm: "j' < m" by auto
+  note updates = add(5)[OF i' j'm]
+  show "d\<mu> fs' i' j' = ?new_mu i' j'" 
+  proof (cases "i' = i")
+    case False
+    thus ?thesis using d i' j' unfolding d\<mu>_def updates by auto
+  next
+    case True
+    have id': "d fs' (Suc j') = d fs (Suc j')" by (rule d, insert i' j', auto)
+    show ?thesis
+      by (rule int_via_rat_eqI, 
+          unfold if_distrib[of rat_of_int] of_int_diff of_int_mult updates id' 
+          d\<mu>[OF add(1) j' i'] d\<mu>[OF Linv j' i'] 
+          if_distrib[of "( * ) (rat_of_int (d fs (Suc j')))"] ring_distribs,
+          insert True i' j' i j d\<mu>[OF Linv], auto simp: gs.\<mu>.simps[of _ x x for x]) 
+  qed
+qed
+
+end
+
+context LLL_with_assms
+begin
+lemma d_d\<mu>_swap: assumes inv: "LLL_invariant False i fs"
+  and i: "i < m"
+  and i0: "i \<noteq> 0" 
+  and norm_ineq: "sq_norm (gso fs (i - 1)) > \<alpha> * sq_norm (gso fs i)" 
+  and fs'_def: "fs' = fs[i := fs ! (i - 1), i - 1 := fs ! i]" 
+shows (* d-updates *)
+  "\<And> ii. ii \<le> m \<Longrightarrow>
+      d fs' ii = (
+        if ii = i then 
+          (d fs (Suc i) * d fs (i - 1) + d\<mu> fs i (i - 1) * d\<mu> fs i (i - 1)) div d fs i 
+        else d fs ii)"
+and (* d\<mu>-updates *)
+  "\<And> ii j. ii < m \<Longrightarrow> j < ii \<Longrightarrow> 
+      d\<mu> fs' ii j = (
+        if ii = i - 1 then 
+           d\<mu> fs i j
+        else if ii = i \<and> j \<noteq> i - 1 then 
+             d\<mu> fs (i - 1) j
+        else if ii > i \<and> j = i then
+           (d fs (Suc i) * d\<mu> fs ii (i - 1) - d\<mu> fs i (i - 1) * d\<mu> fs ii j) div d fs i
+        else if ii > i \<and> j = i - 1 then 
+           (d\<mu> fs i (i - 1) * d\<mu> fs ii j + d\<mu> fs ii i * d fs (i - 1)) div d fs i
+        else d\<mu> fs ii j)" 
+    (is "\<And> ii j. _ \<Longrightarrow> _ \<Longrightarrow> _ = ?new_mu ii j")
+proof -
+  note swap = basis_reduction_swap[OF inv i i0 norm_ineq fs'_def]
+  from i i0 have ii: "i - 1 < i" and le_m: "i - 1 \<le> m" "i \<le> m" "Suc i \<le> m" by auto
+  from LLL_invD[OF inv] have len: "length fs = m" by auto
+  let ?r = rat_of_int
+  let ?n = "\<lambda> i. sq_norm (gso fs i)" 
+  let ?n' = "\<lambda> i. sq_norm (gso fs' i)" 
+  let ?dn = "\<lambda> i. ?r (d fs i * d fs i) * ?n i" 
+  let ?dn' = "\<lambda> i. ?r (d fs' i * d fs' i) * ?n' i" 
+  let ?dmu = "\<lambda> i j. ?r (d fs (Suc j)) * \<mu> fs i j" 
+  let ?dmu' = "\<lambda> i j. ?r (d fs' (Suc j)) * \<mu> fs' i j" 
+  note dmu = d\<mu>[OF inv]
+  note dmu' = d\<mu>[OF swap(1)]
+  note inv' = LLL_invD[OF inv]
+  have nim1: "?n i + square_rat (\<mu> fs i (i - 1)) * ?n (i - 1) = 
+    ?n' (i - 1)" by (subst swap(4), insert i, auto)
+  have ni: "?n i * (?n (i - 1) / ?n' (i - 1)) = ?n' i"
+    by (subst swap(4)[of i], insert i i0, auto)
+  have mu': "\<mu> fs i (i - 1) * (?n (i - 1) / ?n' (i - 1)) = \<mu> fs' i (i - 1)"
+    by (subst swap(5), insert i i0, auto)
+  have fi: "fs ! (i - 1) = fs' ! i" "fs ! i = fs' ! (i - 1)" 
+    unfolding fs'_def using inv'(7) i i0 by auto
+  let ?d'i = "(d fs (Suc i) * d fs (i - 1) + d\<mu> fs i (i - 1) * d\<mu> fs i (i - 1)) div (d fs i)" 
+  have rat': "ii < m \<Longrightarrow> j < ii \<Longrightarrow> ?r (d\<mu> fs' ii j) = ?dmu' ii j" for ii j 
+    using d\<mu>[OF swap(1), of j ii] by simp
+  have rat: "ii < m \<Longrightarrow> j < ii \<Longrightarrow> ?r (d\<mu> fs ii j) = ?dmu ii j"
+      for ii j using d\<mu>[OF inv, of j ii] by simp
+  from i0 i have sim1: "Suc (i - 1) = i" and im1: "i - 1 < m" by auto
+  from LLL_d_Suc[OF inv im1, unfolded sim1] 
+  have dn_im1: "?dn (i - 1) = ?r (d fs i) * ?r (d fs (i - 1))" by simp
+  note pos = Gramian_determinant[OF inv le_refl] 
+  from pos(2) have "?r (gs.Gramian_determinant fs m) \<noteq> 0" by auto
+  from this[unfolded pos(1)] have nzero: "ii < m \<Longrightarrow> ?n ii \<noteq> 0" for ii by auto
+  note pos = Gramian_determinant[OF swap(1) le_refl] 
+  from pos(2) have "?r (gs.Gramian_determinant fs' m) \<noteq> 0" by auto
+  from this[unfolded pos(1)] have nzero': "ii < m \<Longrightarrow> ?n' ii \<noteq> 0" for ii by auto
+  have dzero: "ii \<le> m \<Longrightarrow> d fs ii \<noteq> 0" for ii using LLL_d_pos[OF inv, of ii] by auto
+  have dzero': "ii \<le> m \<Longrightarrow> d fs' ii \<noteq> 0" for ii using LLL_d_pos[OF swap(1), of ii] by auto
+
+  {
+    define start where "start = ?dmu' i (i - 1)" 
+    have "start = (?n' (i - 1) / ?n (i - 1) * ?r (d fs i)) * \<mu> fs' i (i - 1)" 
+      using start_def swap(6)[of i] i i0 by simp
+    also have "\<mu> fs' i (i - 1) = \<mu> fs i (i - 1) * (?n (i - 1) / ?n' (i - 1))" 
+      using mu' by simp
+    also have "(?n' (i - 1) / ?n (i - 1) * ?r (d fs i)) * \<dots> = ?r (d fs i) * \<mu> fs i (i - 1)" 
+      using nzero[OF im1] nzero'[OF im1] by simp
+    also have "\<dots> = ?dmu i (i - 1)" using i0 by simp
+    finally have "?dmu' i (i - 1) = ?dmu i (i - 1)" unfolding start_def .
+  } note dmu_i_im1 = this
+  { (* d updates *)
+    fix j
+    assume j: "j \<le> m" 
+    define start where "start = d fs' j" 
+    {
+      assume jj: "j \<noteq> i" 
+      have "?r start = ?r (d fs' j)" unfolding start_def ..
+      also have "?r (d fs' j) = ?r (d fs j)" 
+        by (subst swap(6), insert j jj, auto)
+      finally have "start = d fs j" by simp
+    } note d_j = this 
+    {
+      assume jj: "j = i"  
+      have "?r start = ?r (d fs' i)" unfolding start_def unfolding jj by simp
+      also have "\<dots> = ?n' (i - 1) / ?n (i - 1) * ?r (d fs i)" 
+        by (subst swap(6), insert i, auto)
+      also have "?n' (i - 1) = (?r (d fs i) / ?r (d fs i)) * (?r (d fs i) / ?r (d fs i)) 
+          * (?n i  + \<mu> fs i (i - 1) * \<mu> fs i (i - 1) * ?n (i - 1))" 
+        by (subst swap(4)[OF im1], insert dzero[of i], insert i, simp)
+      also have "?n (i - 1) = ?r (d fs i) / ?r (d fs (i - 1))" 
+        unfolding LLL_d_Suc[OF inv im1, unfolded sim1] using dzero[of "i - 1"] i0 i by simp
+      finally have "?r start = 
+          ((?r (d fs i) * ?n i) * ?r (d fs (i - 1)) + ?dmu i (i - 1) * ?dmu i (i - 1)) 
+          / (?r (d fs i))" 
+        using i0 dzero[of i] i dzero[of "i - 1"]
+        by (simp add: ring_distribs)
+      also have "?r (d fs i) * ?n i = ?r (d fs (Suc i))" 
+        unfolding LLL_d_Suc[OF inv i] by simp
+      also have "?dmu i (i - 1) = ?r (d\<mu> fs i (i - 1))" by (subst rat, insert i i0, auto)
+      finally have "?r start = (?r (d fs (Suc i) * d fs (i - 1) + d\<mu> fs i (i - 1) * d\<mu> fs i (i - 1)))
+          / (?r (d fs i))" by simp
+      from division_to_div[OF this]
+      have "start = ?d'i" .
+    } note d_i = this
+    from d_j d_i show "d fs' j = (if j = i then ?d'i else d fs j)" unfolding start_def by auto
+  } 
+  have "length fs' = m" 
+    using fs'_def inv'(7) by auto
+  {
+    fix ii j
+    assume ii: "ii < m" and j: "j < ii" 
+    from j ii have sj: "Suc j \<le> m" by auto
+    note swaps = swap(5)[OF ii j] swap(6)[OF sj]
+    show "d\<mu> fs' ii j = ?new_mu ii j" 
+    proof (cases "ii < i - 1")
+      case small: True
+      hence id: "?new_mu ii j = d\<mu> fs ii j" by auto
+      show ?thesis using swaps small ii j i i0 by (auto simp: d\<mu>_def)
+    next
+      case False
+      from j ii have sj: "Suc j \<le> m" by auto
+      let ?start = "d\<mu> fs' ii j" 
+      define start where "start = ?start" 
+      note rat'[OF ii j]
+      note rat_ii_j = rat[OF ii j]
+      from False consider (I) "ii = i" "j = i - 1" | (Is) "ii = i" "j \<noteq> i - 1" | 
+          (Im1) "ii = i - 1" | (large) "ii > i" by linarith
+      thus ?thesis
+      proof cases
+        case iii: Is
+        show ?thesis unfolding swaps d\<mu>_def using iii ii i i0 by auto
+      next
+        case iii: I
+        show ?thesis using dmu_i_im1 rat_ii_j iii i0 by (auto simp: d\<mu>_def)
+      next
+        case iii: Im1
+        show ?thesis unfolding swaps d\<mu>_def using iii ii i j i0 by auto
+      next
+        case iii: large
+        consider (jj) "j \<noteq> i - 1" "j \<noteq> i" | (ji) "j = i" | (jim1) "j = i - 1" by linarith
+        thus ?thesis 
+        proof cases
+          case jj
+          show ?thesis unfolding swaps d\<mu>_def using iii ii i j jj i0 by auto
+        next
+          case ji
+          have "?r start = ?dmu' ii j" unfolding start_def by fact
+          also have "?r (d fs' (Suc j)) = ?r (d fs (Suc i))" unfolding swaps unfolding ji by simp 
+          also have "\<mu> fs' ii j = \<mu> fs ii (i - 1) - \<mu> fs i (i - 1) * \<mu> fs ii i" 
+            unfolding swaps unfolding ji using i0 iii by auto
+          also have "?r (d fs (Suc i)) * \<dots> = ?r (d fs (Suc i)) * ?r (d fs i) / ?r (d fs i) * \<dots>" 
+            using dzero[of i] i by auto
+          also have "\<dots> =  
+            (?r (d fs (Suc i)) * ?dmu ii (i - 1) - ?dmu i (i - 1) * ?dmu ii i) / ?r (d fs i)" 
+            using i0 by (simp add: field_simps)
+          also have "\<dots> = 
+            (?r (d fs (Suc i)) * ?r (d\<mu> fs ii (i - 1)) - ?r (d\<mu> fs i (i - 1)) * ?r (d\<mu> fs ii i)) / ?r (d fs i)" 
+            by (subst (1 2 3) rat, insert i i0 ii iii, auto)
+          also have "\<dots> = ?r (d fs (Suc i) * d\<mu> fs ii (i - 1) - d\<mu> fs i (i - 1) * d\<mu> fs ii i) / ?r (d fs i)" 
+            (is "_ = of_int ?x / _")
+            by simp
+          finally have "?r start = ?r ?x / ?r (d fs i)" .
+          from division_to_div[OF this]
+          have id: "?start = (d fs (Suc i) * d\<mu> fs ii (i - 1) - d\<mu> fs i (i - 1) * d\<mu> fs ii j) div d fs i" 
+            unfolding start_def ji .
+          show ?thesis unfolding id using iii ji by simp
+        next
+          case jim1
+          hence id'': "(j = i - 1) = True" "(j = i) = False" using i0 by auto
+          have "?r (start) = ?dmu' ii j" unfolding start_def by fact
+          also have "\<mu> fs' ii j = \<mu> fs ii (i - 1) * \<mu> fs' i (i - 1) +
+                             \<mu> fs ii i * ?n i / ?n' (i - 1)" (is "_ = ?x1 + ?x2")
+            unfolding swaps unfolding jim1 using i0 iii by auto
+          also have "?r (d fs' (Suc j)) * (?x1 + ?x2)
+              = ?r (d fs' (Suc j)) * ?x1 + ?r (d fs' (Suc j)) * ?x2" by (simp add: ring_distribs)
+          also have "?r (d fs' (Suc j)) * ?x1 = ?dmu' i (i - 1) * (?r (d fs i) * \<mu> fs ii (i - 1))
+            / ?r (d fs i)"
+            unfolding jim1 using i0 dzero[of i] i by simp
+          also have "?dmu' i (i - 1) = ?dmu i (i - 1)" by fact
+          also have "?r (d fs i) * \<mu> fs ii (i - 1) = ?dmu ii (i - 1)" using i0 by simp
+          also have "?r (d fs' (Suc j)) = ?n' (i - 1) * ?r (d fs i) / ?n (i - 1)" 
+            unfolding swaps unfolding jim1 using i0 i by simp 
+          also have "\<dots> * ?x2 = (?n i * ?r (d fs i)) / ?n (i - 1) * \<mu> fs ii i" 
+            using i0 nzero'[of "i - 1"] i by simp
+          also have "?n i * ?r (d fs i) = ?r (d fs (Suc i))" unfolding LLL_d_Suc[OF inv i] ..
+          also have "?r (d fs (Suc i)) / ?n (i - 1) * \<mu> fs ii i = ?dmu ii i / ?n (i - 1)" by simp
+          also have "\<dots> = ?dmu ii i * ?r (d fs (i - 1) * d fs (i - 1)) / ?dn (i - 1)" 
+            using dzero[of "i - 1"] i by simp
+          finally have "?r start = (?dmu i (i - 1) * ?dmu ii j * ?dn (i - 1) + 
+             ?dmu ii i * (?r (d fs (i - 1) * d fs (i - 1) * d fs i))) / (?r (d fs i) * ?dn (i - 1))"
+            unfolding add_divide_distrib of_int_mult jim1
+            using dzero[of "i - 1"] nzero[of "i - 1"] i dzero[of i] by auto
+          also have "\<dots> = (?r (d\<mu> fs i (i - 1)) * ?r (d\<mu> fs ii j) * (?r (d fs i) * ?r (d fs (i - 1))) + 
+             ?r (d\<mu> fs ii i) * (?r (d fs (i - 1) * d fs (i - 1) * d fs i))) / (?r (d fs i) * (?r (d fs i) * ?r (d fs (i - 1))))" 
+            unfolding dn_im1 
+            by (subst (1 2 3) rat, insert i ii iii i0 j, auto)
+          also have "\<dots> = (?r (d\<mu> fs i (i - 1)) * ?r (d\<mu> fs ii j) + ?r (d\<mu> fs ii i) * ?r (d fs (i - 1))) 
+              / ?r (d fs i)" 
+            unfolding of_int_mult using dzero[of i] dzero[of "i - 1"] i i0 by (auto simp: field_simps)
+          also have "\<dots> = ?r (d\<mu> fs i (i - 1) * d\<mu> fs ii j + d\<mu> fs ii i * d fs (i - 1)) / ?r (d fs i)" 
+            (is "_ = of_int ?x / _" )
+            by simp
+          finally have "?r start = ?r ?x / ?r (d fs i)" .
+          from division_to_div[OF this]
+          have id: "?start = (d\<mu> fs i (i - 1) * d\<mu> fs ii j + d\<mu> fs ii i * d fs (i - 1)) div (d fs i)" 
+            unfolding start_def .
+          show ?thesis unfolding id using iii jim1 i0 by auto
+        qed
+      qed
+    qed
+  }
+qed
+
+end
+end
